rename "term" to "program"

theories/Interp.v
@@ -3,7 +3,7 @@ Require Import Unicode.Utf8 Program.Equality Program.Tactics Program.Basics Vect
 From mathcomp Require Import ssreflect.
 Set Bullet Behavior "Strict Subproofs".
 
-From gctt Require Import Notation Term Axioms Var Sequent Tower ExternalSyn.
+From gctt Require Import Notation Program Axioms Var Sequent Tower ExternalSyn.
 From gctt Require Tactic.
 Module T := Tactic.
 
@@ -25,27 +25,27 @@ Notation "κ ∷ σ" := (Env.cons κ σ) (at level 30).
 
 Reserved Notation "⟦ e ⟧ κs" (at level 50).
 
-Fixpoint interp_tm `(e : ETm.t Λ Ψ) (κs : Env.t Λ) : Tm.t Ψ :=
+Fixpoint interp_tm `(e : EProg.t Λ Ψ) (κs : Env.t Λ) : Prog.t Ψ :=
   match e with
-  | ETm.var i => Tm.var i
-  | ETm.fst e => ⟦e⟧ κs .1
-  | ETm.snd e => ⟦e⟧ κs .2
-  | ETm.unit => 𝟙
-  | ETm.bool => 𝟚
-  | ETm.ax => ★
-  | ETm.tt => Tm.tt
-  | ETm.ff => Tm.ff
-  | ETm.prod A B => ⟦A⟧ κs × ⟦B⟧ κs
-  | ETm.arr A B => (⟦A⟧ κs) ⇒ ⟦B⟧ κs
-  | ETm.pair A B => ⟨⟦A⟧ κs, ⟦B⟧ κs⟩
-  | ETm.ltr r A => ▶[κs r] ⟦A⟧ κs
-  | ETm.isect A => ⋂[κ] ⟦A⟧ κ ∷ κs
-  | ETm.univ i => 𝕌[i]
-  | ETm.fix_ e => 𝛍{⟦e⟧ κs}
-  | ETm.lam e => 𝛌{⟦e⟧ κs}
-  | ETm.app e1 e2 => ⟦e1⟧ κs ⋅ ⟦e2⟧ κs
+  | EProg.var i => Prog.var i
+  | EProg.fst e => ⟦e⟧ κs .1
+  | EProg.snd e => ⟦e⟧ κs .2
+  | EProg.unit => 𝟙
+  | EProg.bool => 𝟚
+  | EProg.ax => ★
+  | EProg.tt => Prog.tt
+  | EProg.ff => Prog.ff
+  | EProg.prod A B => ⟦A⟧ κs × ⟦B⟧ κs
+  | EProg.arr A B => (⟦A⟧ κs) ⇒ ⟦B⟧ κs
+  | EProg.pair A B => ⟨⟦A⟧ κs, ⟦B⟧ κs⟩
+  | EProg.ltr r A => ▶[κs r] ⟦A⟧ κs
+  | EProg.isect A => ⋂[κ] ⟦A⟧ κ ∷ κs
+  | EProg.univ i => 𝕌[i]
+  | EProg.fix_ e => 𝛍{⟦e⟧ κs}
+  | EProg.lam e => 𝛌{⟦e⟧ κs}
+  | EProg.app e1 e2 => ⟦e1⟧ κs ⋅ ⟦e2⟧ κs
   end
-where "⟦ e ⟧ κs" := (interp_tm e%etm κs) : tm_scope.
+where "⟦ e ⟧ κs" := (interp_tm e%etm κs) : prog_scope.
 
 Arguments interp_tm [Λ Ψ] e%etm κs.
 
@@ -73,16 +73,16 @@ Arguments interp_jdg [Λ] J%ejdg.
 Notation "⟦ J ⟧" := (interp_jdg J%ejdg) (at level 50) : type_scope.
 
 
-Definition interp_subst `(σ : @Sub.t (ETm.t Λ) Ψ0 Ψ1) (κs : Env.t Λ) : @Sub.t Tm.t Ψ0 Ψ1 :=
+Definition interp_subst `(σ : @Sub.t (EProg.t Λ) Ψ0 Ψ1) (κs : Env.t Λ) : @Sub.t Prog.t Ψ0 Ψ1 :=
   fun x =>
-    (⟦ σ x ⟧ κs)%tm.
+    (⟦ σ x ⟧ κs)%prog.
 
 Notation "⟦ σ ⟧ κs" := (interp_subst σ%esubst κs) : subst_scope.
 
-Local Open Scope tm_scope.
+Local Open Scope prog_scope.
 Local Open Scope program_scope.
 
-Theorem interp_tm_clk_naturality {Λ1 Λ2 Ψ} (e : ETm.t Λ1 Ψ) (ρ : Ren.t Λ1 Λ2) (κs : Env.t Λ2) :
+Theorem interp_tm_clk_naturality {Λ1 Λ2 Ψ} (e : EProg.t Λ1 Ψ) (ρ : Ren.t Λ1 Λ2) (κs : Env.t Λ2) :
   ⟦ e ⟧ κs ∘ ρ = ⟦ e.⦃ρ⦄ ⟧ κs.
 Proof.
   move: Λ2 ρ κs; elim e => *;
@@ -106,7 +106,7 @@ Proof.
   T.rewrites.
 Qed.
 
-Theorem interp_tm_var_naturality {Λ Ψ0 Ψ1 Ψ2} (e : ETm.t Λ Ψ0) (σ : Sub.t Ψ1 Ψ2) ρ κs :
+Theorem interp_tm_var_naturality {Λ Ψ0 Ψ1 Ψ2} (e : EProg.t Λ Ψ0) (σ : Sub.t Ψ1 Ψ2) ρ κs :
   (⟦ e ⟧ κs) ⫽ (σ ∘ ρ) = (⟦ e.[ρ] ⟧ κs) ⫽ σ.
 Proof.
   move: Ψ1 Ψ2 σ ρ κs.
@@ -119,29 +119,29 @@ Proof.
 Qed.
 
 
-Theorem interp_tm_var_ren_naturality {Λ Ψ0 Ψ1} (e : ETm.t Λ Ψ0) (ρ : Ren.t Ψ0 Ψ1) κs :
+Theorem interp_tm_var_ren_naturality {Λ Ψ0 Ψ1} (e : EProg.t Λ Ψ0) (ρ : Ren.t Ψ0 Ψ1) κs :
   (⟦ e ⟧ κs).[ ρ ] = (⟦ e.[ρ] ⟧ κs).
 Proof.
   by rewrite
-     -(Tm.subst_ret (⟦ e .[ ρ] ⟧ κs))
-     -(Tm.subst_ret (⟦ e ⟧ κs .[ρ]))
-     Tm.subst_ren_coh
+     -(Prog.subst_ret (⟦ e .[ ρ] ⟧ κs))
+     -(Prog.subst_ret (⟦ e ⟧ κs .[ρ]))
+     Prog.subst_ren_coh
      interp_tm_var_naturality.
 Qed.
 
 
-Lemma interp_subst_cong_coh {Λ Ψ0 Ψ1 Ψ2} (σ01 : @Sub.t (ETm.t Λ) Ψ0 Ψ1) (σ12 : @Sub.t Tm.t Ψ1 Ψ2) (κs : Env.t Λ) :
+Lemma interp_subst_cong_coh {Λ Ψ0 Ψ1 Ψ2} (σ01 : @Sub.t (EProg.t Λ) Ψ0 Ψ1) (σ12 : @Sub.t Prog.t Ψ1 Ψ2) (κs : Env.t Λ) :
   (Sub.cong σ12 ◎ ⟦ Sub.cong σ01 ⟧ κs)%subst =
   Sub.cong (σ12 ◎ ⟦ σ01 ⟧ κs)%subst.
 Proof.
   T.eqcd => x.
   dependent induction x.
   - eauto.
-  - Term.simplify_subst.
+  - simplify_subst.
     by rewrite -interp_tm_var_naturality.
 Qed.
 
-Theorem interp_tm_subst_naturality {Λ Ψ0 Ψ1 Ψ2} (e : ETm.t Λ Ψ0) (σ12 : Sub.t Ψ1 Ψ2) (σ01 : Sub.t Ψ0 Ψ1) κs :
+Theorem interp_tm_subst_naturality {Λ Ψ0 Ψ1 Ψ2} (e : EProg.t Λ Ψ0) (σ12 : Sub.t Ψ1 Ψ2) (σ01 : Sub.t Ψ0 Ψ1) κs :
   (⟦ e ⟧ κs) ⫽ (σ12 ◎ ⟦ σ01 ⟧ κs) = (⟦ e ⫽ σ01 ⟧ κs) ⫽ σ12.
 Proof.
   symmetry.
@@ -149,13 +149,13 @@ Proof.
   induction e; eauto; simpl;
   T.rewrites_with
     ltac:(repeat f_equal; try (T.eqcd; intros);
-          try rewrite /interp_subst /ETm.wk_sub;
+          try rewrite /interp_subst /EProg.wk_sub;
           try rewrite interp_subst_cong_coh;
-          Term.simplify_subst;
+          Program.simplify_subst;
           try rewrite -interp_tm_clk_naturality).
 Qed.
 
-Theorem interp_tm_ren_naturality {Λ0 Λ1 Ψ0 Ψ1 Ψ2} (e : ETm.t Λ0 Ψ0) (ρΛ : Ren.t Λ0 Λ1) (ρΨ : Ren.t Ψ0 Ψ1) (σ : Sub.t Ψ1 Ψ2) κs :
+Theorem interp_tm_ren_naturality {Λ0 Λ1 Ψ0 Ψ1 Ψ2} (e : EProg.t Λ0 Ψ0) (ρΛ : Ren.t Λ0 Λ1) (ρΨ : Ren.t Ψ0 Ψ1) (σ : Sub.t Ψ1 Ψ2) κs :
   (⟦ e ⟧ κs ∘ ρΛ) ⫽ (σ ∘ ρΨ) = (⟦ e.⦃ρΛ⦄[ρΨ] ⟧ κs) ⫽ σ.
 Proof.
   symmetry.
@@ -164,13 +164,13 @@ Proof.
 
   T.rewrites_with
     ltac:(repeat f_equal; try (T.eqcd; intros);
-          try rewrite /ETm.wk_sub;
+          try rewrite /EProg.wk_sub;
           try rewrite interp_subst_cong_coh;
-          Term.simplify_subst;
+          simplify_subst;
           try rewrite -interp_tm_clk_naturality;
           try rewrite -Sub.cong_coh_ptwise).
 
   by dependent induction x0.
 Qed.
 
-Local Close Scope tm_scope.
+Local Close Scope prog_scope.
