theories/Tower.v
@@ -3,7 +3,7 @@ Require Import Unicode.Utf8 Program.Equality Program.Tactics Setoids.Setoid omeg
 From mathcomp Require Import ssreflect.
 Set Bullet Behavior "Strict Subproofs".
 
-From gctt Require Import OrderTheory Axioms Term OpSem Closure TypeSystem.
+From gctt Require Import OrderTheory Axioms Program OpSem Closure TypeSystem.
 From gctt Require Tactic.
 
 Module T := Tactic.
@@ -18,7 +18,7 @@ Module Spine.
     | S n =>
       fun X =>
         ∃ (j : nat) (p : j ≤ n),
-          fst X ⇓ Tm.univ j
+          fst X ⇓ Prog.univ j
           ∧ snd X = fun es =>
                       ∃ S, Clo.t (@t j _) (fst es, S) ∧ Clo.t (@t j _) (snd es, S)
     end.
@@ -28,7 +28,7 @@ Module Spine.
       t (S n) =
       fun X =>
         ∃ (j : nat) (p : j ≤ n),
-          fst X ⇓ Tm.univ j
+          fst X ⇓ Prog.univ j
           ∧ snd X =
             fun es =>
               ∃ S, Clo.t (t j) (fst es, S) ∧ Clo.t (t j) (snd es, S).
@@ -136,7 +136,7 @@ Module Spine.
 
   Ltac spine_contradiction :=
     lazymatch goal with
-    | H : Spine.t _ (Tm.univ _, _) |- _ => fail "This is a universe!"
+    | H : Spine.t _ (Prog.univ _, _) |- _ => fail "This is a universe!"
     | H : Spine.t ?n (_, _) |- _ =>
       induction n; Spine.simplify;
       [contradiction | T.destruct_conjs; OpSem.destruct_evals]
