Makefile
@@ -108,7 +108,7 @@ VFILES:=theories/Notation.v\
   theories/TypeSystem.v\
   theories/OrderTheory.v\
   theories/Axioms.v\
-  theories/Term.v\
+  theories/Program.v\
   theories/OpSem.v\
   theories/Closure.v\
   theories/Tower.v\
